Prefetcher/Impl.v
@@ -1,96 +1,72 @@
 Require Import Kami.AllNotations.
 Require Import StdLibKami.Fifo.Ifc.
-Require Import StdLibKami.Prefetcher.FifoTop.Impl.
 Require Import StdLibKami.Prefetcher.FifoTop.Ifc.
 Require Import StdLibKami.Prefetcher.Ifc.
 
 Section Prefetch.
-
   Context `{fifoTopParams : FifoTopParams}.
-  Context `{ImmRes: Kind}.
-  Variable PrivMode : Kind.
+  Context `{prefetcherParams: PrefetcherParams}.
 
-  Class PrefetcherImplParams
-    := {
-         PAddrSz : nat;
-         instFifoTop: FifoTop.Ifc.FifoTop
-       }.
+  Context (fifoTop: FifoTop.Ifc.FifoTop).
 
-  Section withParams.
-    Context `{PrefetcherImplParams}.
+  Local Definition PAddr := Bit PAddrSz.
 
-    Local Definition PAddr := Bit PAddrSz.
+  Local Open Scope kami_expr.
+  Local Open Scope kami_action.
 
-    Local Open Scope kami_expr.
-    Local Open Scope kami_action.
+  Definition flush ty: ActionT ty Void :=
+    @FifoTop.Ifc.flush _ fifoTop ty.
+  
+  Definition getIsCompleting ty: ActionT ty (Maybe VAddr) :=
+    @FifoTop.Ifc.getIsCompleting _ fifoTop ty.
 
-    (* TODO: LLEE: update this *)
-    Definition flush ty: ActionT ty Void :=
-      LET inv: Maybe PAddr <- Invalid;
-      LETA _ <- @FifoTop.Ifc.flush _ instFifoTop ty;
-      (* TODO: shouldn't setIsCompleting be called flush if its needed here? *)
-      (* LETA _ <- FifoTop.Ifc.setIsCompleting instFifoTop inv; *)
-      Retv.
-    
-   Definition getIsCompleting ty: ActionT ty (Maybe VAddr) :=
-     LETA completing: Maybe VAddr <- @FifoTop.Ifc.getIsCompleting _ instFifoTop ty;
-     Ret #completing.
+  Definition resetCompleting ty: ActionT ty Void :=
+    @FifoTop.Ifc.resetCompleting _ fifoTop ty.
 
-    Definition memCallback (ty : Kind -> Type) (reordererRes: ty (PrefetcherReordererRes))
-      :  ActionT ty Void
-      := LET entryData
-           :  PrefetcherFifoEntry
-           <- STRUCT {
-                "vaddr" ::= (#reordererRes @% "vaddr" : VAddr @# ty);
-                "data"  ::= (#reordererRes @% "inst" @% "data" : Inst @# ty)
-              };
-         LET entry
-           :  Maybe PrefetcherFifoEntry
-           <- STRUCT {
-                "valid" ::= #reordererRes @% "inst" @% "valid";
-                "data"  ::= #entryData
-              };
-         LETA _ : Bool <- @FifoTop.Ifc.enq _ instFifoTop ty entry;
-         Retv.
+  Definition memCallback (ty : Kind -> Type) (reordererRes: ty PrefetcherRes)
+    :  ActionT ty Void
+    := LET entryData
+         :  PrefetcherFifoEntry
+         <- STRUCT {
+              "vaddr" ::= (toShortVAddr (#reordererRes @% "vaddr" : VAddr @# ty));
+              "info"  ::= #reordererRes @% "info";
+              "inst"  ::= (#reordererRes @% "inst": Maybe Inst @# ty)
+            };
+       LETA _ <- @FifoTop.Ifc.enq _ fifoTop ty entryData;
+       Retv.
 
-    Definition doPrefetch
-        ty
-        (memReq
-          : ty (PrefetcherReordererReq PAddrSz) ->
-            ActionT ty (@PrefetcherReordererImmRes ImmRes))
-         (prefetcherReq: ty (PrefetcherReq PrivMode PAddrSz))
-      :  ActionT ty Bool
-      := LET reordererReq
-           :  PrefetcherReordererReq PAddrSz
-           <- STRUCT {
-                "paddr"  ::= #prefetcherReq @% "paddr";
-                "vaddr" ::= #prefetcherReq @% "vaddr"
-              };
-         LETA reordererImmRes
-           :  @PrefetcherReordererImmRes ImmRes
-           <- memReq reordererReq;
-         Ret (#reordererImmRes @% "ready").
+  Definition doPrefetch
+      ty
+      (memReq
+        : ty PrefetcherReq ->
+          ActionT ty Bool)
+      (prefetcherReq: ty PrefetcherReq)
+    :  ActionT ty Bool
+    := LETA retval <- memReq prefetcherReq;
+       LET dummy: Void <- $0;
+       LETA _ <- @FifoTop.Ifc.enqOutstanding _ fifoTop _;
+       Ret #retval.
 
-    Definition fetchInstruction ty : ActionT ty DeqRes
-      := LETA res : DeqRes <- @FifoTop.Ifc.deq _ instFifoTop ty;
-         Ret #res.
+  Definition fetchInstruction ty : ActionT ty DeqRes
+    := LETA res : DeqRes <- @FifoTop.Ifc.deq _ fifoTop ty;
+       Ret #res.
 
-    Open Scope kami_scope.
-    Open Scope kami_expr_scope.
+  Definition isFull ty: ActionT ty Bool
+    := @FifoTop.Ifc.isFullOutstanding _ fifoTop _.
 
-    Definition regs: list RegInitT := @FifoTop.Ifc.regs _ instFifoTop.
+  Open Scope kami_scope.
+  Open Scope kami_expr_scope.
 
-    Instance prefetcher
-      :  Prefetcher PrivMode PAddrSz
-      := Build_Prefetcher
-           regs
-           (@FifoTop.Ifc.regFiles fifoTopParams instFifoTop)
-           flush
-           getIsCompleting
-           memCallback
-           fetchInstruction
-           doPrefetch.
+  Definition regs := @FifoTop.Ifc.regs _ fifoTop.
+  Definition regFiles := @FifoTop.Ifc.regFiles _ fifoTop.
 
-  End withParams.
-
+  Instance prefetcher: Prefetcher := {| Prefetcher.Ifc.regs := regs;
+                                        Prefetcher.Ifc.regFiles := regFiles;
+                                        Prefetcher.Ifc.flush := flush;
+                                        Prefetcher.Ifc.getIsCompleting := getIsCompleting;
+                                        Prefetcher.Ifc.resetCompleting := resetCompleting;
+                                        Prefetcher.Ifc.isFull := isFull;
+                                        Prefetcher.Ifc.memCallback := memCallback;
+                                        Prefetcher.Ifc.fetchInstruction := fetchInstruction;
+                                        Prefetcher.Ifc.doPrefetch := doPrefetch |}.
 End Prefetch.
