Prefetcher/Ifc.v
@@ -1,51 +1,29 @@
 Require Import Kami.AllNotations.
 Require Import StdLibKami.Fifo.Ifc.
 Require Import StdLibKami.Prefetcher.FifoTop.Ifc.
-Require Import StdLibKami.Prefetcher.FifoTop.Impl.
+
+Class PrefetcherParams :=
+  { PrivMode: Kind;
+    PAddrSz: nat }.
+                           
 
 Section prefetcher.
   Context `{fifoTopParams : FifoTopParams}.
-  Context `{ImmRes : Kind}.
-  Variable PrivMode : Kind.
-  Variable PAddrSz : nat.
+  Context `{PrefetcherParams}.
 
   Local Definition PAddr := Bit PAddrSz.
 
   Definition PrefetcherReq
     := STRUCT_TYPE {
          "mode"  :: PrivMode;
-         "vaddr" :: VAddr;
-         "paddr" :: PAddr
-       }.
-
-  (*
-    Note: isomorphic to ReordererReq.
-  *)
-  Definition PrefetcherReordererReq
-    := STRUCT_TYPE {
-         "paddr"  :: PAddr;
+         "paddr" :: PAddr;
          "vaddr" :: VAddr
        }.
 
-  (*
-    Note: isomorphic to ReordererImmRes.
-    Note: also isomorphic to ArbiterImmRes.
-  *)
-  Definition PrefetcherReordererImmRes
-    := STRUCT_TYPE {
-         "ready" :: Bool;
-         "info"  :: ImmRes (* Maybe Data *)
-       }.
-
-  (*
-    Note: the entire request is returned by the reorderer so that
-    the prefetcher can store the paddr for latter comparison.
-
-    Note: isomorphic to ReordererRes.
-  *)
-  Definition PrefetcherReordererRes
+  Definition PrefetcherRes
     := STRUCT_TYPE {
          "vaddr" :: VAddr;
+         "info"  :: ImmRes;
          "inst"  :: Maybe Inst
        }.
 
@@ -55,38 +33,26 @@ Section prefetcher.
       regFiles : list RegFileBase;
       
       flush: forall {ty}, ActionT ty Void;
+
       (*
         Returns the address that needs to be fetched to retrieve the
         upper 16 bits of the current instruction's 32 bit word.
       *)
       getIsCompleting: forall {ty}, ActionT ty (Maybe VAddr);
 
-      (* Called by the Reorderer. *)
-      memCallback: forall {ty}, ty PrefetcherReordererRes -> ActionT ty Void;
+      resetCompleting: forall {ty}, ActionT ty Void;
 
-      (*
-        Returns a 32 bit word that contains the current instruction
-        and/or the virtual address that needs to be fetched to
-        retrieve this instruction.
-      *)
+      isFull: forall {ty}, ActionT ty Bool;
+      
+      memCallback: forall {ty}, ty PrefetcherRes -> ActionT ty Void;
+
       fetchInstruction: forall {ty}, ActionT ty DeqRes;
 
-      (*
-        Accepts a function, [memReq], that accepts a physical
-        address, verifies that we can load the given address,
-        loads the address if possible, and returns an error code
-        if appropriate; accepts a virtual address, the physical
-        address associated with the virtual address, loads the
-        data referenced by the virtual address, caches the data,
-        and returns true iff the device accepted the load request.
-
-        TODO: LLEE: same ty.
-      *)
       doPrefetch
         ty
         (memReq
-          : ty PrefetcherReordererReq ->
-              ActionT ty PrefetcherReordererImmRes)
+          : ty PrefetcherReq ->
+              ActionT ty Bool)
         : ty PrefetcherReq -> ActionT ty Bool;
     }.
 End prefetcher.
